coq-minuska/theories/martelli_montanari_tests.v
@@ -1,0 +1,149 @@
+From Minuska Require Import
+    spec
+    empty
+    trivial
+    default_everything
+    martelli_montanari
+.
+
+(*
+These examples are taken directly from the
+Haskell implementation test suite. The Coq
+results differ, but are equivalent. This
+is caused by different picking of elements
+between the implementations. However, the
+resulting mgus of both implementation should
+be directly equal.
+
+The first test is a proof of concept, and the
+second is a sanity check. More tests are pointless,
+because, any mistakes will inherently be found out
+during the proving of the rest of the implementation.
+*)
+
+Instance sm : StaticModel := @DSM mysignature β MyProgramInfo.
+
+Definition dec_paper_input1 : list (TermOver BuiltinOrVar) := [
+    t_term "f"
+        [
+            t_over (bov_variable "x1");
+            t_term "g"
+                [t_term "a" [];
+                    t_term "f"
+                        [ t_over (bov_variable "x5"); t_term "b" [] ]
+                ]
+        ];
+    t_term "f"
+        [
+            t_term "h"
+                [ t_term "c" [] ];
+            t_term "g"
+                [t_over (bov_variable "x2");
+                    t_term "f"
+                        [ t_term "b" []; t_over (bov_variable "x5") ]
+                ]
+        ];
+    t_term "f"
+        [
+            t_term "h"
+                [ t_over (bov_variable "x4") ];
+            t_term "g"
+                [t_over (bov_variable "x6");
+                 t_over (bov_variable "x3")
+                ]
+        ]
+    ]
+.
+
+(* This test primarily shows that TermOver_size is enough on a example. *)
+
+Compute (@dec sm dec_paper_input1).
+
+Definition unify_paper1_input1 : TermOver BuiltinOrVar := (t_term "f" [
+  t_over (bov_variable "x1");
+  t_term "g" [t_over (bov_variable "x2"); t_over (bov_variable "x3")];
+  t_over (bov_variable "x2");
+  t_term "b" []]).
+Definition unify_paper1_input2 : TermOver BuiltinOrVar := (t_term "f" [
+  t_term "g" [t_term "h" [t_term "a" []; t_over (bov_variable "x5")]; t_over (bov_variable "x2")];
+  t_over (bov_variable "x1");
+  t_term "h" [t_term "a" []; t_over (bov_variable "x4")];
+  t_over (bov_variable "x4")]).
+
+(*
+Expected result for the last example is:
+
+"0" -> [t_term "f"
+              [
+                t_over (bov_variable "x1");
+                t_over (bov_variable "x1");
+                t_over (bov_variable "x2");
+                t_over (bov_variable "x4")
+              ]
+      ]
+"x4" -> [t_term "b" []]
+"x2" -> [t_term "h" [t_term "a" []; t_term "b" []]]
+"x1" -> [t_term "g"
+              [t_term "h" [
+                            t_term "a" []; 
+                            t_over (bov_variable "x5")
+                          ];
+               t_over (bov_variable "x3")
+              ]
+        ]
+"x5" -> [t_term "b" []]
+"x3" -> [t_term "h" [t_term "a" []; t_term "b" []]]
+*)
+
+Compute (@unify_terms sm U_listset_ops [unify_paper1_input1; unify_paper1_input2]).
+
+
+Definition mgu_res := 
+  match (@unify_terms sm U_listset_ops [unify_paper1_input1; unify_paper1_input2]) with
+    | Some t => Some (extract_mgu t)
+    | None => None
+  end
+.
+
+(*
+Expected result:
+"0"  -> t_term "f" [t_term "g" [
+                                t_term "h" [
+                                            t_term "a" [];t_term "b" []
+                                           ];
+                                t_term "h" [
+                                            t_term "a" [];
+                                            t_term "b" []
+                                           ]
+                              ];
+                  t_term "g" [
+                                t_term "h" [
+                                            t_term "a" [];
+                                            t_term "b" []
+                                           ];
+                                t_term "h" [
+                                            t_term "a" [];
+                                            t_term "b" []
+                                           ]
+                              ];
+                  t_term "h" [
+                              t_term "a" [];
+                              t_term "b" []
+                             ];
+                  t_term "b" []
+                  ]
+"x1" -> t_term "g" [t_term "h" [
+                                t_term "a" [];
+                                t_term "b" []
+                               ];
+                    t_term "h" [
+                                t_term "a" [];
+                                t_term "b" []
+                               ]
+                   ];
+"x2" -> t_term "h" [t_term "a" [];t_term "b" []]);
+"x3" -> t_term "h" [t_term "a" [];t_term "b" []]);
+"x4" -> t_term "b" []);
+"x5" -> t_term "b" [])]
+ *)
+Compute mgu_res.
